FormalCbgraphs/Incompleteness.lean
@@ -1,0 +1,206 @@
+import FormalCbgraphs.Completeness
+import Mathlib.Tactic.DeriveFintype
+
+@[simp]
+theorem Finset.attach_singleton {α} [DecidableEq α] (a : α) :
+    attach {a} = {⟨a, mem_singleton_self a⟩} := rfl
+
+lemma Graph.Connected.root_or_exists_edge {G : Graph} {Roots Edges v} :
+    G.Connected Roots Edges v → v ∈ Roots ∨ ∃ e ∈ Edges, e.v = v := by
+  intro h
+  cases h with
+  | base _ h => exact Or.inl h
+  | step e _ he => exact Or.inr ⟨e, he, rfl⟩
+
+namespace Counterexample
+
+def R : Type :=
+  WithTop (Fin 5)
+deriving LinearOrder, OrderTop
+
+abbrev R.r0 : R := WithTop.some (0 : Fin 5)
+abbrev R.r1 : R := WithTop.some (1 : Fin 5)
+abbrev R.r2 : R := WithTop.some (2 : Fin 5)
+abbrev R.r3 : R := WithTop.some (3 : Fin 5)
+abbrev R.r4 : R := WithTop.some (4 : Fin 5)
+abbrev R.infty := (⊤ : WithTop (Fin 5))
+
+def f1 : R → R
+| WithTop.some x => if x < 4 then WithTop.some (x + 1) else ⊤
+| none => ⊤
+
+def f2 : R → R
+| WithTop.some x => if x < 3 then WithTop.some (x + 3) else ⊤
+| none => ⊤
+
+def f3 : R → R
+| WithTop.some 2 => ⊤
+| r => f1 r
+
+example : R.r0 < R.r2 := by decide
+example : R.r4 < R.infty := by decide
+example : f1 R.r4 = R.infty := rfl
+example : f3 R.r0 = R.r1 := rfl
+
+inductive V : Type
+| a | b | c | d
+deriving DecidableEq
+
+def N : Network R where
+  V := V
+  neighbors
+  | V.a => ∅
+  | V.b => {V.a}
+  | V.c => {V.a, V.b}
+  | V.d => {V.c}
+  init
+  | V.a => R.r0
+  | _ => R.infty
+  transfer
+  | ⟨V.a, V.b, _⟩
+  | ⟨V.b, V.c, _⟩ => f1
+  | ⟨V.a, V.c, _⟩ => f2
+  | ⟨V.c, V.d, _⟩ => f3
+
+variable {S : Schedule N} (hS : S.Fair)
+
+theorem sem_a : ∀ t, S.sem V.a t = R.r0 := by
+  intro t
+  induction t using Nat.strong_induction_on with | _ t ih
+  cases t with
+  | zero => simp [Schedule.sem, N]
+  | succ t =>
+    simp only [Schedule.sem]
+    split_ifs
+    · simp [N]
+    · apply ih
+      simp
+
+theorem sem_b : ∀ t, S.sem V.b t = R.infty ∨ S.sem V.b t = R.r1 := by
+  intro t
+  induction t using Nat.strong_induction_on with | _ t ih
+  cases t with
+  | zero => simp [Schedule.sem, N]
+  | succ t =>
+    simp only [Schedule.sem]
+    split_ifs
+    · simp [N, sem_a]
+      decide
+    · apply ih
+      simp
+
+theorem sem_c : ∀ t, S.sem V.c t = R.infty ∨ S.sem V.c t = R.r2 ∨ S.sem V.c t = R.r3 := by
+  intro t
+  induction t using Nat.strong_induction_on with | _ t ih
+  cases t with
+  | zero => simp [Schedule.sem, N]
+  | succ t =>
+    simp only [Schedule.sem]
+    split_ifs
+    · simp only [N, Finset.attach_insert, Finset.attach_singleton, Finset.image_singleton,
+        Finset.inf_insert, sem_a, Finset.inf_singleton]
+      generalize S.flow ⟨V.b, V.c, _⟩ _ = t'
+      rcases sem_b (S := S) t' with h | h <;> simp +decide [h]
+    · apply ih
+      simp
+
+theorem sem_d : ∀ t, S.sem V.d t = R.infty ∨ S.sem V.d t = R.r4 := by
+  intro t
+  induction t using Nat.strong_induction_on with | _ t ih
+  cases t with
+  | zero => simp [Schedule.sem, N]
+  | succ t =>
+    simp [Schedule.sem]
+    split_ifs
+    · simp only [N, Finset.attach_singleton, Finset.inf_singleton]
+      generalize S.flow ⟨V.c, V.d, _⟩ _ = t'
+      rcases sem_c (S := S) t' with h | h | h <;> simp +decide [h]
+    · apply ih
+      simp
+
+section
+
+include hS
+
+theorem sem_b_converge : ∃ T, ∀ t ≥ T, S.sem V.b t = R.r1 := by
+  rcases hS.2 ⟨V.a, V.b, by simp [N]⟩ 0 with ⟨T₁, -, h₁⟩
+  rcases hS.1 V.b (T₁ + 1) with ⟨T₂, hT₂, h₂⟩
+  exists T₂
+  intro t ht
+  induction t using Nat.strong_induction_on with | _ t ih
+  cases t with
+  | zero => grind
+  | succ t =>
+    simp only [Schedule.sem]
+    split_ifs
+    · simp +decide [N, sem_a]
+    · apply ih <;> grind
+
+theorem sem_c_converge : ∃ T, ∀ t ≥ T, S.sem V.c t = R.r2 := by
+  rcases sem_b_converge hS with ⟨T₁, h₁⟩
+  rcases hS.2 ⟨V.b, V.c, by simp [N]⟩ T₁ with ⟨T₂, hT₂, h₂⟩
+  rcases hS.1 V.c (T₂ + 1) with ⟨T₃, hT₃, h₃⟩
+  exists T₃
+  intro t ht
+  induction t using Nat.strong_induction_on with | _ t ih
+  cases t with
+  | zero => grind
+  | succ t =>
+    simp only [Schedule.sem]
+    split_ifs
+    · simp only [N, Finset.attach_insert, Finset.attach_singleton, Finset.image_singleton,
+        Finset.inf_insert, sem_a, Finset.inf_singleton]
+      generalize ht' : S.flow ⟨V.b, V.c, _⟩ _ = t'
+      simp +decide [h₁ t' (by rw [← ht']; apply h₂; grind)]
+    · apply ih <;> grind
+
+theorem sem_d_converge : ∃ T, ∀ t ≥ T, S.sem V.d t = R.infty := by
+  rcases sem_c_converge hS with ⟨T₁, h₁⟩
+  rcases hS.2 ⟨V.c, V.d, by simp [N]⟩ T₁ with ⟨T₂, hT₂, h₂⟩
+  rcases hS.1 V.d (T₂ + 1) with ⟨T₃, hT₃, h₃⟩
+  exists T₃
+  intro t ht
+  induction t using Nat.strong_induction_on with | _ t ih
+  cases t with
+  | zero => grind
+  | succ t =>
+    simp only [Schedule.sem]
+    split_ifs
+    · simp only [N, Finset.attach_singleton, Finset.inf_singleton]
+      generalize ht' : S.flow ⟨V.c, V.d, _⟩ _ = t'
+      simp +decide [h₁ t' (by rw [← ht']; apply h₂; grind)]
+    · apply ih <;> grind
+
+end
+
+theorem incomplete : ∃ Y, N.IsEventualStable Y ∧ IsEmpty (VC N Y) := by
+  let Y : N.V → R → Prop | V.d, s => s = R.infty | _, _ => True
+  refine ⟨Y, ?_, ?_⟩
+  · intro S hS v
+    cases v with
+    | a | b | c => simp [Y]
+    | d => simp only [Y]; exact sem_d_converge hS
+  · by_contra! ⟨vc⟩
+    let S := N.syncSchedule
+    have hS : S.Fair := N.fair_syncSchedule
+    have hc : vc.Q V.c R.r2 := by
+      rcases vc.connected_cbgraph hS V.c with ⟨T, h⟩
+      rcases sem_c_converge hS with ⟨T', h'⟩
+      grind [h (max T T'), h' (max T T')]
+    have hd : vc.I V.d R.r4 := by
+      convert vc.invariance (S := S) V.d 2
+      decide +kernel
+    have hd' : ¬ vc.Q V.d R.r4 := by
+      intro h
+      apply vc.property at h
+      revert h
+      decide
+    rcases (vc.connected V.d).root_or_exists_edge with h | ⟨e, h, he⟩
+    · apply hd'
+      convert vc.cbroot (S := S) _ h 2 (by simp)
+      decide +kernel
+    · rcases e with ⟨u, _, hu⟩
+      subst he
+      simp only [N, Finset.mem_singleton] at hu
+      subst hu
+      exact hd' (vc.edge _ h _ _ hc hd)
